Fixes to the invariants, fixes to the scope entering lemmas. Non-trivial admits were left there, to be investigated quicly

coq/LLVMGen/Correctness_Invariants.v
@@ -201,12 +201,13 @@ Section SimulationRelations.
       nth_error σ n ≡ Some (DSHPtrVal addr val) ->
       mem_block_exists addr m.
 
-  Definition no_id_aliasing (s : IRState) (σ : evalContext) : Prop :=
-    forall n n' id τ τ',
-      (* WF_IRState σ s -> *) (* TODO: See if we need this? *)
-      nth_error (Γ s) n ≡ Some (id, τ) ->
-      nth_error (Γ s) n' ≡ Some (id, τ') ->
-      n' ≡ n /\ exists v, nth_error σ n ≡ Some v.
+  Definition no_id_aliasing (σ : evalContext) (s : IRState) : Prop :=
+    forall n1 n2 id τ τ' v1 v2,
+      nth_error σ n1 ≡ Some v1 ->
+      nth_error σ n2 ≡ Some v2 ->
+      nth_error (Γ s) n1 ≡ Some (id, τ) ->
+      nth_error (Γ s) n2 ≡ Some (id, τ') ->
+      n2 ≡ n1. 
 
   Definition no_llvm_ptr_aliasing (σ : evalContext) (s : IRState) (ρ : local_env) (g : global_env) : Prop :=
     forall (id1 : ident) (ptrv1 : addr) (id2 : ident) (ptrv2 : addr) n1 n2 τ τ' v1 v2,
@@ -242,8 +243,8 @@ Section SimulationRelations.
   Lemma incLocal_no_id_aliasing :
     forall s1 s2 id σ,
       incLocal s1 ≡ inr (s2, id) ->
-      no_id_aliasing s1 σ ->
-      no_id_aliasing s2 σ.
+      no_id_aliasing σ s1 ->
+      no_id_aliasing σ s2.
   Proof.
     intros s1 s2 id * INC ALIAS.
     unfold no_id_aliasing in *.
@@ -253,17 +254,16 @@ Section SimulationRelations.
   Qed.
 
   Lemma no_id_aliasing_n_eq :
-    forall s σ n n' id τ τ',
-      no_id_aliasing s σ ->
+    forall s σ n n' id τ τ' v v',
+      no_id_aliasing σ s ->
+      nth_error σ n ≡ Some v ->
+      nth_error σ n' ≡ Some v' ->
       nth_error (Γ s) n ≡ Some (id, τ) ->
       nth_error (Γ s) n' ≡ Some (id, τ') ->
       n' ≡ n.
   Proof.
     intros s σ n n' id τ τ' ALIAS N1 N2.
-    edestruct ALIAS.
-    eapply N1.
-    eapply N2.
-    eauto.
+    edestruct ALIAS; eauto. 
   Qed.
 
   Definition no_local_global_alias (l : local_env) (g : global_env) (v : uvalue) : Prop :=
@@ -400,7 +400,7 @@ Section SimulationRelations.
     {
     mem_is_inv : memory_invariant σ s memH configV ;
     IRState_is_WF : WF_IRState σ s ;
-    st_no_id_aliasing : no_id_aliasing s σ ;
+    st_no_id_aliasing : no_id_aliasing σ s ;
     st_no_dshptr_aliasing : no_dshptr_aliasing σ ;
     st_no_llvm_ptr_aliasing : no_llvm_ptr_aliasing_cfg σ s configV ;
     st_id_allocated : id_allocated σ memH
@@ -604,8 +604,8 @@ Section SimulationRelations.
   Lemma incVoid_no_id_aliasing :
     forall s1 s2 id σ,
       incVoid s1 ≡ inr (s2, id) ->
-      no_id_aliasing s1 σ ->
-      no_id_aliasing s2 σ.
+      no_id_aliasing σ s1 ->
+      no_id_aliasing σ s2.
   Proof.
     intros s1 s2 id SIG INC ALIAS.
     unfold no_id_aliasing in *.
@@ -1170,8 +1170,8 @@ Qed.
 Lemma incLocalNamed_no_id_aliasing :
   forall s1 s2 msg id σ,
     incLocalNamed msg s1 ≡ inr (s2, id) ->
-    no_id_aliasing s1 σ ->
-    no_id_aliasing s2 σ.
+    no_id_aliasing σ s1 ->
+    no_id_aliasing σ s2.
 Proof.
   intros s1 s2 msg id * INC ALIAS.
   unfold no_id_aliasing in *.
@@ -1205,8 +1205,8 @@ Qed.
 Lemma incBlockNamed_no_id_aliasing :
   forall s1 s2 msg id σ,
     incBlockNamed msg s1 ≡ inr (s2, id) ->
-    no_id_aliasing s1 σ ->
-    no_id_aliasing s2 σ.
+    no_id_aliasing σ s1 ->
+    no_id_aliasing σ s2.
 Proof.
   intros s1 s2 msg id * INC ALIAS.
   unfold no_id_aliasing in *.
@@ -1249,9 +1249,9 @@ Qed.
 
 Lemma no_id_aliasing_gamma :
   forall s1 s2 σ,
-    no_id_aliasing s1 σ ->
+    no_id_aliasing σ s1 ->
     Γ s1 ≡ Γ s2 ->
-    no_id_aliasing s2 σ.
+    no_id_aliasing σ s2.
 Proof.
   intros s1 s2 σ ALIAS GAMMA.
   unfold no_id_aliasing.
@@ -1307,203 +1307,182 @@ Proof.
     rewrite EQ in LU.
     rewrite nth_error_Sn in LU;eauto.
 
-  - red; intros * LU1 LU2.
-    specialize (ALIAS1 (S n) (S n')).
+  - red; intros * LU1 LU2 LU3 LU4.
+    specialize (ALIAS1 (S n1) (S n2)).
     rewrite EQ, 2nth_error_Sn in ALIAS1.
     eapply ALIAS1 in LU1; eauto.
-    destruct LU1 as (SN & N).
-    inv SN.
-    auto.
   - red; intros * LU1 LU2.
     specialize (ALIAS2 (S n) (S n')).
     rewrite 2nth_error_Sn in ALIAS2.
     eapply ALIAS2 in LU1; eauto.
 
-  - do 2 red. intros * LU1 LU2 LU3 LU4 INEQ.
+  - do 2 red. intros * LU1 LU2 LU3 LU4 INEQ IN1 IN2.
     do 2 red in ALIAS3.
     specialize (ALIAS3 id1 ptrv1 id2 ptrv2 (S n1) (S n2)).
     rewrite !EQ, !nth_error_Sn in ALIAS3.
     eapply ALIAS3 in LU1; eauto.
-Admitted.
 
-Lemma state_invariant_enter_scope_DSHnat : forall σ v x τ s1 s2 stH mV l g,
-    τ ≡ getWFType x DSHnat ->
-    Γ s1 ≡ (x,τ) :: Γ s2 ->
-    ~ In x (map fst (Γ s2)) ->
-    in_local_or_global_scalar l g mV x (dvalue_of_int v) τ ->
-    state_invariant σ s2 stH (mV,(l,g)) ->
-    state_invariant (DSHnatVal v::σ) s1 stH (mV,(l,g)).
+  - red.
+    intros * LU.
+    eapply (st_id_allocated0 (S n)); eauto.
+Qed.
+
+(* TO MOVE *)
+Definition uvalue_of_nat k := UVALUE_I64 (Int64.repr (Z.of_nat k)).
+
+Lemma state_invariant_enter_scope_DSHnat : 
+  forall σ v prefix x s1 s2 stH mV l g,
+    newLocalVar IntType prefix s1 ≡ inr (s2, x) ->
+    ~ in_Gamma σ s1 x ->
+    l @ x ≡ Some (uvalue_of_nat v) ->
+    state_invariant σ s1 stH (mV,(l,g)) ->
+    state_invariant (DSHnatVal (Int64.repr (Z.of_nat v))::σ) s2 stH (mV,(l,g)).
 Proof.
-  intros * -> EQ fresh IN [MEM WF ALIAS1 ALIAS2 ALIAS3].
+  intros * EQ GAM LU [MEM WF ALIAS1 ALIAS2 ALIAS3]; inv EQ; cbn in *.
   split.
   - red; intros * LU1 LU2.
     destruct n as [| n].
-    + rewrite EQ in LU2; cbn in *.
-      inv LU1; inv LU2; auto.
+    + cbn in *; inv LU1; inv LU2; auto.
+      cbn; rewrite repr_intval; auto.
     + rewrite nth_error_Sn in LU1.
-      rewrite EQ, nth_error_Sn in LU2.
+      cbn in *.
       eapply MEM in LU2; eauto.
   -  do 2 red.
-     intros ? [| n] LU.
-     + cbn in LU.
-       inv LU.
-       rewrite EQ; cbn; eauto.
-     + rewrite nth_error_Sn in LU.
-       rewrite EQ,nth_error_Sn.
-       apply WF in LU; auto.
+     cbn.
+     intros ? [| n] LU'.
+     + cbn in LU'.
+       inv LU'.
+       cbn.
+       exists (ID_Local (Name (prefix @@ string_of_nat (local_count s1)))); reflexivity.
+     + rewrite nth_error_Sn in LU'.
+       rewrite nth_error_Sn.
+       apply WF in LU'; auto.
 
-  - red; intros * LU1 LU2.
-    destruct n as [| n], n' as [| n']; auto.
-    + rewrite EQ in LU2; cbn in *.
-      rewrite EQ in LU1; cbn in *.
-      inv LU1; inv LU2; auto. split; auto. eexists; auto.
+  - red; intros * LU1 LU2 LU3 LU4.
+    destruct n1 as [| n1], n2 as [| n2]; auto.
+    + exfalso. cbn in *.
+      apply GAM.
+      inv LU3; eapply mk_in_Gamma; eauto.
     + exfalso.
-      rewrite EQ, nth_error_Sn in LU2.
-      rewrite EQ in LU1.
-      cbn in *.
-      inv LU1.
-      apply fresh.
-      apply nth_error_In in LU2.
-      replace id with (fst (id,τ')) by reflexivity.
-      apply in_map; auto.
-
-    + exfalso.
-      rewrite EQ, nth_error_Sn in LU1.
-      rewrite EQ in LU2.
-      cbn in *.
-      inv LU2.
-      apply fresh.
-      apply nth_error_In in LU1.
-      replace id with (fst (id,τ)) by reflexivity.
-      apply in_map; auto.
-
-    + rewrite EQ, nth_error_Sn in LU1.
-      rewrite EQ, nth_error_Sn in LU2.
-      eapply ALIAS1 in LU1; apply LU1 in LU2; eauto.
-      destruct LU2; split; auto.
+      apply GAM; inv LU4; eapply mk_in_Gamma; eauto.
+    + inv LU3; inv LU4; eapply ALIAS1 in LU1; apply LU1 in LU2; eauto.
 
   - red; intros * LU1 LU2.
     destruct n as [| n], n' as [| n']; auto.
     + inv LU1.
-
     + inv LU2.
-
-
     + rewrite nth_error_Sn in LU1.
       rewrite nth_error_Sn in LU2.
       eapply ALIAS2 in LU1; apply LU1 in LU2; eauto.
 
-  - do 2 red. intros * LU1 LU2 LU3 LU4 INEQ.
+  - do 2 red. intros * LU1 LU2 LU3 LU4 INEQ IN1 IN2.
+    cbn in *.
     destruct n1 as [| n1], n2 as [| n2]; auto.
-    + cbn in LU1. inv LU1; inv LU2.
-      intros H H0.
-      admit. (* Probably need to make about locals only *)
-    + cbn in *; inv LU1.
-      admit.
-    + cbn in *; inv LU2.
-      admit.
-Admitted.
-
-Lemma state_invariant_enter_scope_DSHCType : forall σ v x τ s1 s2 stH mV l g,
-    τ ≡ getWFType x DSHCType ->
-    Γ s1 ≡ (x,τ) :: Γ s2 ->
-    ~ In x (map fst (Γ s2)) ->
-    in_local_or_global_scalar l g mV x (dvalue_of_bin v) τ ->
-    state_invariant σ s2 stH (mV,(l,g)) ->
-    state_invariant (DSHCTypeVal v::σ) s1 stH (mV,(l,g)).
-Proof.
-  intros * -> EQ fresh IN [MEM WF ALIAS1 ALIAS2 ALIAS3].
-  split.
-  - red; intros * LU1 LU2.
-    destruct n as [| n].
-    + rewrite EQ in LU2; cbn in *.
-      inv LU1; inv LU2; auto.
-    + rewrite nth_error_Sn in LU1.
-      rewrite EQ, nth_error_Sn in LU2.
-      eapply MEM in LU2; eauto.
-  -  do 2 red.
-     intros ? [| n] LU.
-     + cbn in LU.
-       inv LU.
-       rewrite EQ; cbn; eauto.
-     + rewrite nth_error_Sn in LU.
-       rewrite EQ,nth_error_Sn.
-       apply WF in LU; auto.
-
-  - red; intros * LU1 LU2.
-    destruct n as [| n], n' as [| n']; auto.
-    + rewrite EQ in LU2; cbn in *.
-      rewrite EQ in LU1; cbn in *.
-      inv LU1; inv LU2; auto. split; auto. eexists; auto.
-    + exfalso.
-      rewrite EQ, nth_error_Sn in LU2.
-      rewrite EQ in LU1.
+    + cbn in *. inv LU1; inv LU2; inv LU3; inv LU4; auto.
+    + cbn in *; inv LU1; inv LU3; eauto.
       cbn in *.
-      inv LU1.
-      apply fresh.
-      apply nth_error_In in LU2.
-      replace id with (fst (id,τ')) by reflexivity.
-      apply in_map; auto.
-
-    + exfalso.
-      rewrite EQ, nth_error_Sn in LU1.
-      rewrite EQ in LU2.
-      cbn in *.
-      inv LU2.
-      apply fresh.
-      apply nth_error_In in LU1.
-      replace id with (fst (id,τ)) by reflexivity.
-      apply in_map; auto.
-
-    + rewrite EQ, nth_error_Sn in LU1.
-      rewrite EQ, nth_error_Sn in LU2.
-      eapply ALIAS1 in LU1; apply LU1 in LU2; eauto.
-      destruct LU2; split; auto.
-
-  - red; intros * LU1 LU2.
-    destruct n as [| n], n' as [| n']; auto.
-    + inv LU1.
-
-    + inv LU2.
-
-
-    + rewrite nth_error_Sn in LU1.
-      rewrite nth_error_Sn in LU2.
-      eapply ALIAS2 in LU1; apply LU1 in LU2; eauto.
-
-  - do 2 red. intros * LU1 LU2 LU3 LU4 INEQ.
-    destruct n1 as [| n1], n2 as [| n2]; auto.
+      rewrite LU in IN1; inv IN1.
+    + cbn in *; inv LU2; inv LU4.
+      cbn in *; rewrite LU in IN2; inv IN2.
     + cbn in *.
-      inv LU1; inv LU2.
-      admit.
-    + cbn in *; inv LU1.
-      admit.
-    + cbn in *; inv LU2.
-      admit.
-Admitted.
+      eapply ALIAS3; [exact LU1 | exact LU2 |..]; eauto.
+  - intros [| n] * LUn; [inv LUn |].
+    eapply st_id_allocated0; eauto.
+Qed.
+
+(* TO FIX *)
+(* Lemma state_invariant_enter_scope_DSHCType : forall σ v x τ s1 s2 stH mV l g, *)
+(*     τ ≡ getWFType x DSHCType -> *)
+(*     Γ s1 ≡ (x,τ) :: Γ s2 -> *)
+(*     ~ In x (map fst (Γ s2)) -> *)
+(*     in_local_or_global_scalar l g mV x (dvalue_of_bin v) τ -> *)
+(*     state_invariant σ s2 stH (mV,(l,g)) -> *)
+(*     state_invariant (DSHCTypeVal v::σ) s1 stH (mV,(l,g)). *)
+(* Proof. *)
+(*   intros * -> EQ fresh IN [MEM WF ALIAS1 ALIAS2 ALIAS3]. *)
+(*   split. *)
+(*   - red; intros * LU1 LU2. *)
+(*     destruct n as [| n]. *)
+(*     + rewrite EQ in LU2; cbn in *. *)
+(*       inv LU1; inv LU2; auto. *)
+(*     + rewrite nth_error_Sn in LU1. *)
+(*       rewrite EQ, nth_error_Sn in LU2. *)
+(*       eapply MEM in LU2; eauto. *)
+(*   -  do 2 red. *)
+(*      intros ? [| n] LU. *)
+(*      + cbn in LU. *)
+(*        inv LU. *)
+(*        rewrite EQ; cbn; eauto. *)
+(*      + rewrite nth_error_Sn in LU. *)
+(*        rewrite EQ,nth_error_Sn. *)
+(*        apply WF in LU; auto. *)
+
+(*   - red; intros * LU1 LU2 LU3 LU4. *)
+(*     destruct n1 as [| n1], n2 as [| n2]; auto. *)
+(*     + exfalso. *)
+(*       inv LU3; apply GAM. *)
+(*       apply nth_error_In in LU2. *)
+(*       replace id with (fst (id,τ')) by reflexivity. *)
+(*       apply in_map; auto. *)
+
+(*     + exfalso. *)
+(*       rewrite EQ, nth_error_Sn in LU1. *)
+(*       rewrite EQ in LU2. *)
+(*       cbn in *. *)
+(*       inv LU2. *)
+(*       apply fresh. *)
+(*       apply nth_error_In in LU1. *)
+(*       replace id with (fst (id,τ)) by reflexivity. *)
+(*       apply in_map; auto. *)
+
+(*     + rewrite EQ, nth_error_Sn in LU1. *)
+(*       rewrite EQ, nth_error_Sn in LU2. *)
+(*       eapply ALIAS1 in LU1; apply LU1 in LU2; eauto. *)
+(*       destruct LU2; split; auto. *)
+
+(*   - red; intros * LU1 LU2. *)
+(*     destruct n as [| n], n' as [| n']; auto. *)
+(*     + inv LU1. *)
+
+(*     + inv LU2. *)
+
+
+(*     + rewrite nth_error_Sn in LU1. *)
+(*       rewrite nth_error_Sn in LU2. *)
+(*       eapply ALIAS2 in LU1; apply LU1 in LU2; eauto. *)
+
+(*   - do 2 red. intros * LU1 LU2 LU3 LU4 INEQ. *)
+(*     destruct n1 as [| n1], n2 as [| n2]; auto. *)
+(*     + cbn in *. *)
+(*       inv LU1; inv LU2. *)
+(*       admit. *)
+(*     + cbn in *; inv LU1. *)
+(*       admit. *)
+(*     + cbn in *; inv LU2. *)
+(*       admit. *)
+(* Admitted. *)
 
 Lemma state_invariant_enter_scope_DSHPtr :
   forall σ ptrh sizeh ptrv x τ s1 s2 stH mV mV_a l g,
     τ ≡ getWFType (ID_Local x) (DSHPtr sizeh) ->
-    Γ s1 ≡ (ID_Local x,τ) :: Γ s2 ->
+    Γ s2 ≡ (ID_Local x,τ) :: Γ s1 ->
 
     (* Freshness *)
-    ~ In (ID_Local x) (map fst (Γ s2)) ->          (* The new ident is fresh *)
+    ~ in_Gamma σ s1 x ->
+    (* ~ In (ID_Local x) (map fst (Γ s2)) ->          (* The new ident is fresh *) *)
     (forall sz, ~ In (DSHPtrVal ptrh sz) σ) -> (* The new Helix address is fresh *)
-    no_llvm_ptr_aliasing_cfg σ s2 (mV, (l, g)) ->
-
-    state_invariant σ s2 stH (mV,(l,g)) ->
 
     (* We know that a certain ptr has been allocated *)
-    allocate mV (DTYPE_Array (Z.to_N (Int64.intval sizeh)) DTYPE_Double) ≡
-             inr (mV_a, ptrv) ->
+    allocate mV (DTYPE_Array (Z.to_N (Int64.intval sizeh)) DTYPE_Double) ≡ inr (mV_a, ptrv) ->
 
-    state_invariant (DSHPtrVal ptrh sizeh :: σ) s1
+    state_invariant σ s1 stH (mV,(l,g)) ->
+
+    state_invariant (DSHPtrVal ptrh sizeh :: σ) s2
                     (memory_set stH ptrh mem_empty)
                     (mV_a, (alist_add x (UVALUE_Addr ptrv) l,g)).
 Proof.
   Opaque add_logical_block. Opaque next_logical_key.
-  intros * -> EQ fresh1 fresh2 fresh3 [MEM WF ALIAS1 ALIAS2 ALIAS3] alloc.
+  intros * -> EQ GAM fresh alloc [MEM WF ALIAS1 ALIAS2 ALIAS3 ALLOC].
   split.
   - red; intros * LU1 LU2.
     destruct n as [| n].
@@ -1530,8 +1509,9 @@ Proof.
     + rewrite nth_error_Sn in LU1.
       rewrite EQ, nth_error_Sn in LU2.
       eapply MEM in LU2; eauto.
-      (* Why do we have an admit here now? TO FIX *)
+  (* There is some reasoning on the memory (on [alloc] in particular) to be done here *)
       admit.
+
   - do 2 red.
     intros ? [| n] LU.
     + cbn in LU.
@@ -1542,54 +1522,34 @@ Proof.
       rewrite EQ,nth_error_Sn.
       apply WF in LU; auto.
 
-  - red; intros * LU1 LU2.
-    destruct n as [| n], n' as [| n']; auto.
-    + rewrite EQ in LU2; cbn in *.
-      rewrite EQ in LU1; cbn in *.
-      inv LU1; inv LU2; auto. split; auto. eexists; auto.
+  - red; intros * LU1 LU2 LU3 LU4.
+    destruct n1 as [| n1], n2 as [| n2]; auto.
 
     + exfalso.
-      rewrite EQ, nth_error_Sn in LU2.
-      rewrite EQ in LU1.
-      cbn in *.
-      inv LU1.
-      apply fresh1.
-      apply nth_error_In in LU2.
-      replace (ID_Local x) with (fst (ID_Local x,τ')) by reflexivity.
-      apply in_map; auto.
-
+      inv LU1; rewrite EQ in LU3; inv LU3.
+      rewrite EQ in LU4.
+      cbn in LU2.
+      cbn in LU4.
+      apply GAM; eapply mk_in_Gamma; eauto.
+ 
     + exfalso.
-      rewrite EQ, nth_error_Sn in LU1.
-      rewrite EQ in LU2.
-      cbn in *.
-      inv LU2.
-      apply fresh1.
-      apply nth_error_In in LU1.
-      replace (ID_Local x) with (fst (ID_Local x,τ)) by reflexivity.
-      apply in_map; auto.
+      inv LU2; rewrite EQ in LU4; inv LU4.
+      rewrite EQ in LU3.
+      apply GAM; eapply mk_in_Gamma; eauto.
 
-    + rewrite EQ in LU2; cbn in *.
-      rewrite EQ in LU1; cbn in *.
-      inv LU1; inv LU2; auto.
-      split.
-      assert (n ≡ n'). {
-        eapply ALIAS1; eauto.
-      } subst; auto.
-      admit.
+    + rewrite EQ in LU3,LU4; cbn in *.
+      f_equal. eapply ALIAS1; eauto.
 
   - red; intros * LU1 LU2.
     destruct n as [| n], n' as [| n']; auto.
     + cbn in *. inv LU1. exfalso.
-      eapply fresh2.
+      eapply fresh.
       apply nth_error_In in LU2. eauto.
     + cbn in *. inv LU2. exfalso.
-      eapply fresh2.
+      eapply fresh.
       apply nth_error_In in LU1. eauto.
     + cbn in *.
-      assert (n ≡ n'). {
-        eapply ALIAS2; eauto.
-      }
-      subst; auto.
+      f_equal; eapply ALIAS2; eauto.
 
   - do 2 red. intros * LU1 LU2 LU3 LU4 INEQ IN1 IN2.
     destruct n1 as [| n1], n2 as [| n2]; auto.
@@ -1599,28 +1559,41 @@ Proof.
       inv LU1; inv LU2; inv LU3; inv LU4.
       eauto.
     + rewrite EQ in LU3,LU4.
+      Opaque allocate.
+      clear MEM.
       cbn in *.
       inv LU1; inv LU3.
-      (* eapply fresh3 in IN1; eauto. *)
-      (* red in IN1, IN. *)
-      (* destruct id1; cbn; eauto. *)
-      (* rewrite IN1 in IN; inv IN; auto. *)
-      (* rewrite IN1 in IN; inv IN; auto. *)
-      admit.
+      cbn in *.
+      rewrite alist_find_add_eq in IN1; inv IN1.
+      red in ALLOC.
+      (* - ptrv1 is fresh in [mV] by alloc
+         - ptrv2 was already loaded in a variable stored in Gamma: it _should_ therefore has already been allocated.
+         -> do I already have the intel to prove that?
+         TO FIGURE OUT
+       *)
+
+     admit.
     + rewrite EQ in LU3,LU4.
+      Opaque allocate.
+      clear MEM.
       cbn in *.
       inv LU2; inv LU4.
-      (* eapply fresh3 in IN1; eauto. *)
-      (* red in IN2, IN. *)
-      (* destruct id2; cbn; eauto. *)
-      (* rewrite IN2 in IN; inv IN; auto. *)
-      (* rewrite IN2 in IN; inv IN; auto. *)
+      cbn in *.
+      rewrite alist_find_add_eq in IN2; inv IN2.
+      red in ALLOC.
+      (* - ptrv2 is fresh in [mV] by alloc
+         - ptrv1 was already loaded in a variable stored in Gamma: it _should_ therefore has already been allocated.
+         -> do I already have the intel to prove that?
+         TO FIGURE OUT
+       *)
+
       admit.
     + rewrite EQ in LU3,LU4.
       cbn in *.
       eapply ALIAS3.
       apply LU1.
       all:eauto.
+      admit.
 Admitted.
 
 Lemma vellvm_helix_ptr_size:
