coq/LLVMGen/Correctness_Alloc.v
@@ -276,30 +276,8 @@ Proof.
           apply genIR_local_count in genIR_op'. cbn in *.
           split; try split; try split; eauto. reflexivity.
         }
-        intro. apply H.
-        eapply In_nth_error in H3; destruct H3.
-        destruct (nth_error (Γ s1) x) eqn: nth_destruct.
-        2 : {
-          eapply map_nth_error_none in nth_destruct.
-          rewrite nth_destruct in H3.
-          inversion H3.
-        }
-
-        destruct p.
-
-        red in st_no_id_aliasing.
-        specialize (st_no_id_aliasing _ _ _ _ _ nth_destruct nth_destruct).
-        destruct st_no_id_aliasing as (? & ? & X).
-
-        esplit.
-        2 : {
-          rewrite nth_destruct.
-          eapply map_nth_error in nth_destruct.
-          rewrite nth_destruct in H3. cbn in H3; inversion H3; subst.
-          reflexivity.
-        }
-        2 : auto. exact X.
-      - (* ∀ s : Int64.int, ¬ List.In (DSHPtrVal (memory_next_key memH) s) σ *)
+        auto.
+     - (* ∀ s : Int64.int, ¬ List.In (DSHPtrVal (memory_next_key memH) s) σ *)
         intros. (* Use fact about memory_next_key *)
         pose proof @mem_block_exists_memory_next_key.
         destruct PRE.
@@ -308,8 +286,6 @@ Proof.
         intro. apply H.
         apply In_nth_error in H3. destruct H3.
         eapply st_id_allocated. apply H3.
-      - destruct PRE. clear -st_no_llvm_ptr_aliasing.
-        eauto.
     }
 
     Transparent incBlockNamed.
@@ -350,6 +326,7 @@ Proof.
 
     split; red; cbn; repeat break_let; subst.
     cbn in *.
+    (* TODO: avoid inlining this proof, figure out why it's true and derive it from a lemma *)
     destruct state_PRE. cbn in mem_is_inv.
     split.
     - cbn. intros. rewrite context_l0 in mem_is_inv.
@@ -378,9 +355,9 @@ Proof.
       specialize (IRState_is_WF v (S n)). cbn in IRState_is_WF. apply IRState_is_WF in H4.
       apply H4.
     - red. cbn in *. intros. red in st_no_id_aliasing.
-      rewrite context_l0 in st_no_id_aliasing. specialize (st_no_id_aliasing (S n) (S n')).
-      cbn in *. specialize (st_no_id_aliasing _ _ _ H4 H5). destruct st_no_id_aliasing.
-      inv H1. split; auto.
+      rewrite context_l0 in st_no_id_aliasing. specialize (st_no_id_aliasing (S n1) (S n2)).
+      cbn in *. specialize (st_no_id_aliasing _ _ _ _ _ H4 H5 H6 H7).
+      inv st_no_id_aliasing; auto.
     - unfold no_dshptr_aliasing in *. intros.
       specialize (st_no_dshptr_aliasing (S n) (S n')).
       cbn in st_no_dshptr_aliasing.
